src/frontend/Main.fst
@@ -14,6 +14,7 @@ let test =
     let decls = Simplify.simplify_prog env decls in
     // FStar.IO.print_string (String.concat "\n" (List.map Ast.print_decl decls));
     let t_decls = List.map Translate.translate_decl decls in
-    FStar.IO.print_string (Target.print_decls t_decls)
+    FStar.IO.print_string (Target.print_decls t_decls);
+    FStar.IO.print_string (Target.print_c_entry t_decls)
   | _ ->
     failwith "Not enough arguments"
